theories/Contract_monae_redesign.v
@@ -1,0 +1,372 @@
+(* This Source Code Form is subject to the terms of the Mozilla Public
+ * License, v. 2.0. If a copy of the MPL was not distributed with this
+ * file, You can obtain one at https://mozilla.org/MPL/2.0/. *)
+
+(* Copyright (C) 2018–2020 ANSSI *)
+
+(** In this library, we provide the necessary material to reason about FreeSpec
+    components both in isolation, and in composition.  To do that, we focus our
+    reasoning principles on interfaces, by defining how their primitives shall
+    be used, and what to expect the result computed by “correct” operational
+    semantics (according to a certain definition of “correct”). *)
+
+From Stdlib Require Import Setoid Morphisms.
+(* From ExtLib Require Import StateMonad MonadState MonadTrans. *)
+From FreerDPS Require Import Interface Impure Semantics Component.
+From mathcomp Require Import ssreflect.
+From monae Require Import preamble hierarchy.
+#[local]
+Open Scope signature_scope.
+Open Scope monae_scope.
+
+Generalizable All Variables.
+
+(** * Definition *)
+
+(** A contract_m dedicated to [i : interface] primarily provides two
+    predicates.
+
+    - [caller_obligation] distinguishes between primitives that can be used (by
+      an impure computation), and primitives that cannot be used.
+    - [callee_obligation] specifies which guarantees can be expected from
+      primitives results, as computed by a “good” operational semantics.
+
+    Both [caller_obligation] and [callee_obligation] model properties that may
+    vary in time, e.g., a primitive may be forbidden at a given time, but
+    authorized later.  To take this possibility into account, contracts are
+    parameterized by what we have called a “witness.”  A witness is a term which
+    describes the necessary information of the past, and allows for taking
+    decision for the present.  It can be seen as an abstraction of the concrete
+    state of the interface implementor.
+
+    To keep this state up-to-date after each primitive interpretation,
+    contracts also define a dedicated function [witness_update]. *)
+Record contract_m (i : interface) (M : monad) (Ω : UU0) : UU0 :=
+  make_contract_m
+  { witness_update :
+      Ω -> forall α, i α -> M α -> forall b, M b
+
+  ; caller_obligation :
+      Ω -> forall α, i α -> Prop
+
+  ; callee_obligation :
+      Ω -> forall α, i α -> M α -> Prop
+  }.
+
+  Declare Scope contract_scope.
+Bind Scope contract_scope with contract_m.
+
+Arguments make_contract_m [i M Ω] (_ _ _).
+Check witness_update _ _ _ _.
+Arguments witness_update [i M Ω] (c ω) [α] (_ _).
+Arguments caller_obligation [i M Ω] (c ω) [α] (_).
+Arguments callee_obligation [i M Ω] (c ω) [α] (_ _).
+
+(* ========================================================================= *)
+Section s_contract.
+  Context {M : monad}. 
+  Definition const_witness {i} ()  := fun (_ : unit) a (e : i a) (m : M a) b => @skip M.
+
+Inductive no_caller_obligation {i} {Ω} (ω : Ω) (α : Type) (e : i α) : Prop :=
+| mk_no_caller_obligation : no_caller_obligation ω α e.
+
+Hint Constructors no_caller_obligation : freespec.
+
+Inductive no_callee_obligation {i Ω} (ω : Ω) (α : Type) (e : i α) (x : M α) : Prop :=
+| mk_no_callee_obligation : no_callee_obligation ω α e x.
+
+Hint Constructors no_callee_obligation : freespec.
+
+Definition no_contract (i : interface) : contract_m i M unit :=
+  {| witness_update := const_witness
+   ; caller_obligation := no_caller_obligation
+   ; callee_obligation := no_callee_obligation
+   |}.
+
+(** A similar —and as simple— contract is the one that forbids the use of a
+    given interface. *)
+
+Definition do_no_use {i Ω} (ω : Ω) (α : Type) (e : i α) : Prop := False.
+
+Definition forbid_specs (i : interface) : contract_m i M unit :=
+  {| witness_update := const_witness
+   ; caller_obligation := do_no_use
+   ; callee_obligation := no_callee_obligation
+   |}.
+
+End s_contract.
+
+(* ========================================================================= *)
+
+Definition contract_m_caller_equ
+    `(c1 : contract_m i M Ω1)
+    `(c2 : contract_m i M Ω2)
+    (f : Ω1 -> Ω2)
+  : Prop :=
+  forall ω1 α (p : i α),
+    caller_obligation c1 ω1 p <->
+    caller_obligation c2 (f ω1) p.
+
+Definition contract_m_callee_equ
+    `(c1 : contract_m i M Ω1)
+    `(c2 : contract_m i M Ω2)
+    (f : Ω1 -> Ω2)
+  : Prop :=
+  forall ω1 α (p : i α) (mx : M α),
+    callee_obligation c1 ω1 p mx <->
+    callee_obligation c2 (f ω1) p mx.
+
+Definition contract_m_witness_equ
+    `(c1 : contract_m i M Ω1)
+    `(c2 : contract_m i M Ω2)
+    (f : Ω1 -> Ω2)
+  : Prop :=
+  forall ω1 α (p : i α) (mx : M α),
+    f (witness_update c1 ω1 p mx)
+      =
+    witness_update c2 (f ω1) p mx.
+
+
+Inductive contract_m_equ `(c1 : contract_m i M Ω1) `(c2 : contract_m i M Ω2)
+  : Type :=
+| mk_contract_m_equ (f : Ω1 -> Ω2) (g : Ω2 -> Ω1)
+    (iso1 : forall x, f (g x) = x) (iso2 : forall x, g (f x) = x)
+    (caller_equ : contract_m_caller_equ c1 c2 f)
+    (callee_equ : contract_m_callee_equ c1 c2 f)
+    (witness_equ : contract_m_witness_equ c1 c2 f)
+  : contract_m_equ c1 c2.
+
+Definition contract_m_iso_lr `(c1 : contract_m i M Ω1) `(c2 : contract_m i M Ω2)
+    (equ : contract_m_equ c1 c2) (ω1 : Ω1)
+  : Ω2 :=
+  match equ with
+  | @mk_contract_m_equ _ _ _ _ _ _ f _ _ _ _ _ _ => f ω1
+  end.
+
+Definition contract_m_iso_rl `(c1 : contract_m i M Ω1) `(c2 : contract_m i M Ω2)
+    (equ : contract_m_equ c1 c2) (ω2 : Ω2)
+  : Ω1 :=
+  match equ with
+  | @mk_contract_m_equ _ _ _ _ _ _ _ g _ _ _ _ _ => g ω2
+  end.
+
+Arguments contract_m_iso_lr {i M Ω1 c1 Ω2 c2} (equ ω1).
+Arguments contract_m_iso_rl {i M Ω1 c1 Ω2 c2} (equ ω2).
+
+Lemma contract_m_equ_refl `(c : contract_m i M Ω)
+  : contract_m_equ c c.
+
+Proof.
+  apply mk_contract_m_equ with (f:=fun x => x) (g:=fun x => x); auto.
+  + now intros ω α p.
+  + now intros ω α p x.
+  + now intros ω α p x.
+Defined.
+
+Lemma contract_m_equ_sym `(c1 : contract_m i M Ω1) `(c2 : contract_m i M Ω2)
+   (equ : contract_m_equ c1 c2)
+  : contract_m_equ c2 c1.
+
+Proof.
+  induction equ.
+  apply mk_contract_m_equ with (f:=g) (g:=f).
+  + apply iso2.
+  + apply iso1.
+  + intros ω α p.
+    transitivity (caller_obligation c2 (f (g ω)) p).
+    ++ now rewrite iso1.
+    ++ now symmetry.
+  + intros ω α p x.
+    transitivity (callee_obligation c2 (f (g ω)) p x).
+    ++ now rewrite iso1.
+    ++ now symmetry.
+  + intros ω α p x.
+    rewrite <- (iso2 (witness_update c1 (g ω) p x)).
+    assert (equ : witness_update c2 ω p x = f (witness_update c1 (g ω) p x)). {
+      transitivity (witness_update c2 (f (g ω)) p x).
+      + now rewrite iso1.
+      + now rewrite witness_equ.
+    }
+    now rewrite equ.
+Defined.
+
+Lemma contract_m_equ_trans `(c1 : contract_m i M Ω1) `(c2 : contract_m i M Ω2)
+   `(c3 : contract_m i M Ω3)
+   `(is_equ12 : contract_m_equ c1 c2)
+   `(is_equ23 : contract_m_equ c2 c3)
+  : contract_m_equ c1 c3.
+
+Proof.
+  destruct is_equ12 as [f12 g21 isofg12 isogf12 caller_equ12 callee_equ12 witness_equ12].
+  destruct is_equ23 as [f23 g32 isofg23 isogf23 caller_equ23 callee_equ23 witness_equ23].
+  apply mk_contract_m_equ
+    with (f:=fun x => f23 (f12 x)) (g:=fun x => g21 (g32 x)).
+  + setoid_rewrite isofg12.
+    now setoid_rewrite isofg23.
+  + setoid_rewrite isogf23.
+    now setoid_rewrite isogf12.
+  + intros ω1 α p.
+    transitivity (caller_obligation c2 (f12 ω1) p);
+      [ now apply caller_equ12
+      | now apply caller_equ23 ].
+  + intros ω1 α p x.
+    transitivity (callee_obligation c2 (f12 ω1) p x); [ now apply callee_equ12
+                                                      | now apply callee_equ23 ].
+  + intros ω1 α p x.
+    rewrite <- witness_equ23.
+    assert (equ : f12 (witness_update c1 ω1 p x) = witness_update c2 (f12 ω1) p x)
+      by now rewrite <- witness_equ12.
+    now rewrite equ.
+Defined.
+
+(* ========================================================================= *)
+
+Definition gen_witness_update
+    `{MayProvide ix i}
+    {Ω α}
+    {M : monad}
+    (c : contract_m i M Ω)
+    (ω : Ω)
+    (e : ix α)
+    (mx : M α)
+  : Ω :=
+  match proj_p e with
+  | Some e => witness_update c ω e mx
+  | None   => ω
+  end.
+
+Definition gen_caller_obligation `{MayProvide ix i} {Ω α} {M : monad} (c : contract_m i M Ω)
+    (ω :  Ω) (e : ix α)
+  : Prop :=
+  match proj_p e with
+  | Some e => caller_obligation c ω e
+  | None => True
+  end.
+
+Definition gen_callee_obligation
+    `{MayProvide ix i}
+    {Ω α}
+    {M : monad}
+    (c : contract_m i M Ω)
+    (ω : Ω)
+    (e : ix α)
+    (mx : M α)
+  : Prop :=
+  match proj_p e with
+  | Some e => callee_obligation c ω e mx
+  | None   => True
+  end.
+
+(* ========================================================================= *)
+
+  Definition contract_mprod
+    `{Provide ix i, Provide ix j}
+    {M : monad}
+    {Ωi Ωj}
+    (ci : contract_m i M Ωi)
+    (cj : contract_m j M Ωj)
+  : contract_m ix M (Ωi * Ωj):=
+  {| witness_update := fun (ω : Ωi * Ωj) (α : Type) (e : ix α) (x : M α) =>
+                         (gen_witness_update ci (fst ω) e x, gen_witness_update cj (snd ω) e x)
+  ;  caller_obligation := fun (ω : Ωi * Ωj) (α : Type) (e : ix α) =>
+                       gen_caller_obligation ci (fst ω) e /\ gen_caller_obligation cj (snd ω) e
+  ;  callee_obligation := fun (ω : Ωi * Ωj) (α : Type) (e : ix α) (x : M α) =>
+                   gen_callee_obligation ci (fst ω) e x /\ gen_callee_obligation cj (snd ω) e x
+  |}.
+
+Infix "*" := contract_mprod : contract_scope.
+
+Definition sharedcontractprod `{Provide ix i, Provide ix j} {M: monad}
+   `(ci : contract_m i M Ω) (cj : contract_m j M Ω)
+  : contract_m ix M Ω :=
+  {|
+  witness_update :=
+    fun (ω : Ω) (α : Type) (e : ix α) (x : M α) =>
+      (* we need to check [i] before [j] because [sharedcontractprod]
+         will be right associative *)
+      match proj_p (i:=i) e with
+      | Some e => witness_update ci ω e x
+      | _ => match proj_p (i:=j) e with
+             | Some e => witness_update cj ω e x
+             | _ => ω
+             end
+      end;
+  caller_obligation :=
+    fun (ω : Ω) (α : Type) (e : ix α) =>
+      gen_caller_obligation ci ω e /\ gen_caller_obligation cj ω e;
+  callee_obligation :=
+    fun (ω : Ω) (α : Type) (e : ix α) (x : M α) =>
+      gen_callee_obligation ci ω e x /\ gen_callee_obligation cj ω e x
+  |}.
+
+Infix "^" := sharedcontractprod  : contract_scope.
+
+(* ========================================================================= *)
+
+Section s_store.
+  Context (S : UU0) {M : stateMonad S}.
+Check witness_update.
+(*      : forall (i : interface) (M : monad) (Ω : UU0), contract_m i M Ω -> Ω -> forall α : UU0, i α -> M α -> Ω *)
+Definition store_update : S -> forall α : UU0, STORE S α -> M α -> M α.
+move => x A e m.
+inversion e; subst. 
+- apply/get.
+- apply/put/x0.
+Defined.
+
+Inductive o_callee_store (x : S) : forall (α : Type), STORE S α -> M α -> Prop :=
+| get_o_callee (x' : M S) (equ : Ret x = x') : o_callee_store x S Get x'
+| put_o_callee (x' : S) (u : M unit) : o_callee_store x unit (Put x') u.
+
+Definition store_specs : contract_m (STORE S) M S :=
+  {| witness_update := store_update
+  ;  caller_obligation := no_caller_obligation
+  ;  callee_obligation := o_callee_store
+  |}.
+
+Definition store_update (s : Type) {M : stateMonad s} . :=
+  fun (x : s) (α : Type) (e : STORE s α) (_ : M α) =>
+    match e with
+    | Get => get
+    | Put x' => put x'
+    end.
+
+  Check store_update.
+  Check stateMonad.
+
+(** Assuming the mutable variable is being initialized prior to any impure
+    computation interpretation, we do not have any obligations over the use of
+    [STORE s] primitives.  We will get back to this assertion once we have
+    defined our contract, but in the meantime, we define its callee obligation.
+
+    The logic of these callee obligations is as follows: [Get] is expected to
+    produce a result strictly equivalent to the witness, and we do not have any
+    obligations about the result of [Put] (which belongs to [unit] anyway, so
+    there is not much to tell). *)
+
+Inductive o_callee_store (s : Type) (x : s) : forall (α : Type), STORE s α -> α -> Prop :=
+| get_o_callee (x' : s) (equ : x = x') : o_callee_store s x s Get x'
+| put_o_callee (x' : s) (u : unit) : o_callee_store s x unit (Put x') u.
+
+(** The actual contract can therefore be defined as follows: *)
+
+Definition store_specs (s : Type) : contract (STORE s) s :=
+  {| witness_update := store_update s
+  ;  caller_obligation := no_caller_obligation
+  ;  callee_obligation := o_callee_store s
+  |}.
+
+(** Now, as we briefly mentionned, this contract allows for reasoning about an
+    impure computation which uses the [STORE s] interface, assuming the mutable,
+    global variable has been initialized.  We can define another contract that
+    does not rely on such assumption, and on the contrary, requires an impure
+    computation to initialize the variable prior to using it.
+
+    In this context, the witness can solely be a boolean which tells if the
+    variable has been initialized, and the [callee_obligation] will require the
+    witness to be [true] to authorize a call of [Get].
+
+    This is one of the key benefits of the FreeSpec approach: because the
+    contracts are defined independently from impure computations and
+    interfaces, we can actually define several contracts to consider
+    different set of hypotheses. *)
